@prefix : <http://www.ai4eu.eu/ontologies/core#> .
@prefix dct: <http://purl.org/dc/terms/> .
@prefix owl: <http://www.w3.org/2002/07/owl#> .
@prefix rdf: <http://www.w3.org/1999/02/22-rdf-syntax-ns#> .
@prefix xml: <http://www.w3.org/XML/1998/namespace> .
@prefix xsd: <http://www.w3.org/2001/XMLSchema#> .
@prefix foaf: <http://xmlns.com/foaf/0.1/> .
@prefix rdfs: <http://www.w3.org/2000/01/rdf-schema#> .
@base <http://www.ai4eu.eu/ontologies/core> .

<http://www.ai4eu.eu/ontologies/core> rdf:type owl:Ontology ;
                                       owl:versionIRI <http://www.ai4eu.eu/ontologies/0.1/core> ;
                                       #owl:imports foaf: ;
                                       dct:date "2021-02-18"@en ;
                                       rdfs:comment "The AI4EU ontology aims to formally represent the AI4EU model for describing AI resources"@en ;
                                       rdfs:label "The AI4EU Ontology"@en ;
                                       owl:versionInfo "0.9.5"@en .

#################################################################
#    Annotation properties
#################################################################

###  http://purl.org/dc/terms/date
dct:date rdf:type owl:AnnotationProperty .


#################################################################
#    Object Properties
#################################################################

###  http://www.ai4eu.eu/ontologies/core#accompanied_by
:accompanied_by rdf:type owl:ObjectProperty ;
                rdfs:domain :Distribution ;
                rdfs:range :Documentation ;
                rdfs:comment "Associates a resource distribution with a documentation item for the resource."@en ;
                rdfs:label "Accompanied by"@en .


###  http://www.ai4eu.eu/ontologies/core#associated_with
:associated_with rdf:type owl:ObjectProperty ;
                 rdfs:domain :AIResource ;
                 rdfs:range foaf:Project ;
                 rdfs:comment "Associates an AI resource with a project relevant to the resource."@en ;
                 rdfs:label "Associated With"@en .


###  http://www.ai4eu.eu/ontologies/core#atTRL
:atTRL rdf:type owl:ObjectProperty ;
       rdfs:domain :Distribution ;
       rdfs:range :TechnologyReadinessLevel ;
       rdfs:comment "Associates a distribution of an AI resource with its technology readiness level."@en ;
       rdfs:label "At TRL"@en .


###  http://www.ai4eu.eu/ontologies/core#authority
:authority rdf:type owl:ObjectProperty ;
           rdfs:domain :TechnologyReadinessLevel ;
           rdfs:range foaf:Agent ;
           rdfs:comment "Associates a Technology Readiness Level with the organisation that defined it."@en ;
           rdfs:label "Authority"@en .


###  http://www.ai4eu.eu/ontologies/core#distributed_as
:distributed_as rdf:type owl:ObjectProperty ;
                rdfs:domain :AIResource ;
                rdfs:range :Distribution ;
                rdfs:comment "Associates an AI resource with one of its distributions"@en ;
                rdfs:label "Distributed as"@en .


###  http://www.ai4eu.eu/ontologies/core#language_used
:language_used rdf:type owl:ObjectProperty ;
               rdfs:domain :Distribution ;
               rdfs:comment "The programming language primarily used for/by an AI resource."@en ;
               rdfs:label "Language Used"@en .


###  http://www.ai4eu.eu/ontologies/core#location
:location rdf:type owl:ObjectProperty ;
          rdfs:domain foaf:Organization ;
          rdfs:comment "The country where an organisation participating in the development or management of a resource is located. It is recommended that the DBPedia URI of the corresponding country is provided."@en ;
          rdfs:label "Location"@en .


###  http://www.ai4eu.eu/ontologies/core#organised_by
:organised_by rdf:type owl:ObjectProperty ;
          rdfs:domain :Challenge ;
          rdfs:range :Project ;
          rdfs:comment "The Project that organised the challenge."@en ;
          rdfs:label "Organised by"@en .


###  http://www.ai4eu.eu/ontologies/core#provider
:provider rdf:type owl:ObjectProperty ;
          rdfs:domain :Distribution ;
          rdfs:range foaf:Agent ;
          rdfs:comment "An entity responsible for the creation/distribution of a resource."@en ;
          rdfs:label "Provider"@en .


###  http://www.ai4eu.eu/ontologies/core#refers_to
:refers_to rdf:type owl:ObjectProperty ;
           rdfs:domain :AIResource ;
           rdfs:range <http://www.w3.org/2004/02/skos/core#Concept> ;
           rdfs:comment "Associates an AI resource with the AI fields it adheres to."@en ;
           rdfs:label "Refers to"@en .


###  http://www.ai4eu.eu/ontologies/core#requires
:requires rdf:type owl:ObjectProperty ;
          rdfs:domain :AIResource ;
          rdfs:range :ComputationalResource ;
          rdfs:comment "Associates an AI resource with the computational resources it requires for functioning."@en ;
          rdfs:label "Requires"@en .


###  http://www.ai4eu.eu/ontologies/core#used_in
:used_in rdf:type owl:ObjectProperty ;
         rdfs:domain :AIResource ;
         rdfs:range :ApplicationArea ;
         rdfs:comment "Associates an AI resource with its application areas."@en ;
         rdfs:label "Used in"@en .


#################################################################
#    Data properties
#################################################################

###  http://www.ai4eu.eu/ontologies/core#acumos_distribution
:acumos_distribution rdf:type owl:DatatypeProperty ;
                     rdfs:domain :Distribution ;
                     rdfs:range xsd:anyURI ;
                     rdfs:comment "Associates a resource with its distribution in the AI4EU Acumos deployment."@en ;
                     rdfs:label "Acumos Distribution"@en .


###  http://www.ai4eu.eu/ontologies/core#download
:download rdf:type owl:DatatypeProperty ;
          rdfs:domain :Distribution ;
          rdfs:range xsd:anyURI ;
          rdfs:comment "A web address from where a distribution is made available."@en ;
          rdfs:label "Download"@en .


###  http://www.ai4eu.eu/ontologies/core#trl
:trl rdf:type owl:DatatypeProperty ;
     rdfs:domain :TechnologyReadinessLevel ;
     rdfs:range xsd:integer ;
     rdfs:comment "Associates a Technology Readiness Level instance with the corresponding numeric value."@en ;
     rdfs:label "TRL Value"@en .


###  http://www.ai4eu.eu/ontologies/core#under_license
:under_license rdf:type owl:DatatypeProperty ;
               rdfs:domain :Distribution ;
               rdfs:range xsd:anyURI ;
               rdfs:comment "Associates a resource distribution with its accompanying license."@en ;
               rdfs:label "Under License"@en .


#################################################################
#    Classes
#################################################################

###  http://www.ai4eu.eu/ontologies/core#AIOrganization
:AIOrganization rdf:type owl:Class ;
                rdfs:subClassOf :KnowledgeComponent ,
                                foaf:Organization ;
                rdfs:comment "An organization with interest or expertise in AI technologies"@en ;
                rdfs:label "AI Organization"@en .


###  http://www.ai4eu.eu/ontologies/core#AIResource
:AIResource rdf:type owl:Class ;
            rdfs:subClassOf :Entity ;
            rdfs:comment "An accessible and usable resource pertaining to AI research and applications."@en ;
            rdfs:label "AI Resource"@en .


###  http://www.ai4eu.eu/ontologies/core#Application
:Application rdf:type owl:Class ;
             rdfs:subClassOf :StandAlone ;
             rdfs:comment "A distribution directly executable on the user's hardware"@en ;
             rdfs:label "Application"@en .


###  http://www.ai4eu.eu/ontologies/core#ApplicationArea
:ApplicationArea rdf:type owl:Class ;
                 rdfs:subClassOf :Quality ;
                 rdfs:comment "An application or scientific domain where an AI resource is or can be of use (possibly in the context of a larger framework)."@en ;
                 rdfs:label "Application Area"@en .


###  http://www.ai4eu.eu/ontologies/core#Challenge
:Challenge rdf:type owl:Class ;
           rdfs:subClassOf :KnowledgeComponent ;
           rdfs:comment "A challenge organised in the context of an Event or Project."@en ;
           rdfs:label "Challenge"@en .


###  http://www.ai4eu.eu/ontologies/core#Company
:Company rdf:type owl:Class ;
         rdfs:subClassOf :Entity ,
                         foaf:Organization ;
         rdfs:comment "A private institution or corporation."@en ;
         rdfs:label "Company"@en .


###  http://www.ai4eu.eu/ontologies/core#ComputationalResource
:ComputationalResource rdf:type owl:Class ;
                       rdfs:subClassOf :Entity ;
                       rdfs:comment "A hardware or software asset to be used by other entities like programs or models."@en ;
                       rdfs:label "Computational Resource"@en .


###  http://www.ai4eu.eu/ontologies/core#Dataset
:Dataset rdf:type owl:Class ;
         rdfs:subClassOf :KnowledgeComponent ;
         rdfs:comment "A collection of data."@en ;
         rdfs:label "Dataset"@en .


###  http://www.ai4eu.eu/ontologies/core#Distribution
:Distribution rdf:type owl:Class ;
              rdfs:subClassOf :Entity ;
              rdfs:comment "A specific form of packaging and means of exposure and availability for an AI resource."@en ;
              rdfs:label "Distribution"@en .


###  http://www.ai4eu.eu/ontologies/core#DockerContainer
:DockerContainer rdf:type owl:Class ;
                 rdfs:subClassOf :StandAlone ;
                 rdfs:comment "A standalone distribution of an AI resource, bundled as a Docker container"@en ;
                 rdfs:label "Docker Container"@en .


###  http://www.ai4eu.eu/ontologies/core#Documentation
:Documentation rdf:type owl:Class ;
               rdfs:subClassOf :Entity ;
               rdfs:comment "An entity that provides further information on the characteristics and usage of an AI Resource"@en ;
               rdfs:label "Documentation"@en .


###  http://www.ai4eu.eu/ontologies/core#EducationalResource
:EducationalResource rdf:type owl:Class ;
                     rdfs:subClassOf :KnowledgeComponent ;
                     rdfs:comment "A resource built and distributed for educational purposes"@en ;
                     rdfs:label "Educational Resource"@en .


###  http://www.ai4eu.eu/ontologies/core#Embedded
:Embedded rdf:type owl:Class ;
          rdfs:subClassOf :Distribution ;
          rdfs:comment "A distribution of an AI resource that is engrained into a broader solution or system."@en ;
          rdfs:label "Embedded"@en .


###  http://www.ai4eu.eu/ontologies/core#Entity
:Entity rdf:type owl:Class ;
        rdfs:comment "An AI-related concept that has a tangible manifestation (i.e. it has a physical or digital presence)"@en ;
        rdfs:label "Entity"@en .


###  http://www.ai4eu.eu/ontologies/core#Event
:Event rdf:type owl:Class ;
       rdfs:subClassOf :KnowledgeComponent ;
       rdfs:comment "A happening of note for the broader AI community"@en ;
       rdfs:label "Event"@en .


###  http://www.ai4eu.eu/ontologies/core#Forum
:Forum rdf:type owl:Class ;
       rdfs:subClassOf :Website ;
       rdfs:comment "A website where users can exchange information and feedback on an AI resource."@en ;
       rdfs:label "Forum"@en .


###  http://www.ai4eu.eu/ontologies/core#HardwareComponent
:HardwareComponent rdf:type owl:Class ;
                   rdfs:subClassOf :AIResource ;
                   rdfs:comment "A hardware AI resource (device/equipment)."@en ;
                   rdfs:label "Hardware Component"@en .


###  http://www.ai4eu.eu/ontologies/core#KnowledgeComponent
:KnowledgeComponent rdf:type owl:Class ;
                    rdfs:subClassOf :AIResource ;
                    rdfs:comment "A resource that encapsulates knowledge or results relevant to AI research and applications."@en ;
                    rdfs:label "Knowledge Component"@en .


###  http://www.ai4eu.eu/ontologies/core#Library
:Library rdf:type owl:Class ;
         rdfs:subClassOf :Distribution ;
         rdfs:comment "A distribution meant to be incorporated as a module into a larger framework or application."@en ;
         rdfs:label "Library"@en .


###  http://www.ai4eu.eu/ontologies/core#Manual
:Manual rdf:type owl:Class ;
        rdfs:subClassOf :Documentation ;
        rdfs:comment "A document that provides instructions on the installation, management or usage of an AI resource."@en ;
        rdfs:label "Manual"@en .


###  http://www.ai4eu.eu/ontologies/core#Model
:Model rdf:type owl:Class ;
       rdfs:subClassOf :KnowledgeComponent ;
       rdfs:comment "An AI Model."@en ;
       rdfs:label "Model"@en .


###  http://www.ai4eu.eu/ontologies/core#ModelBundle
:ModelBundle rdf:type owl:Class ;
             rdfs:subClassOf :Distribution ;
             rdfs:comment "Distribution of an AI resource in an Acumos-ready onboarding format."@en ;
             rdfs:label "Model Bundle"@en .


###  http://www.ai4eu.eu/ontologies/core#Notebook
:Notebook rdf:type owl:Class ;
          rdfs:subClassOf :Distribution ;
          rdfs:comment "Distribution of an AI resource as a digital notebook (e.g. Jupyter)"@en ;
          rdfs:label "Notebook"@en .


###  http://www.ai4eu.eu/ontologies/core#Ontology
:Ontology rdf:type owl:Class ;
          rdfs:subClassOf :KnowledgeComponent ;
          rdfs:label "Ontology"@en .


###  http://www.ai4eu.eu/ontologies/core#Presentation
:Presentation rdf:type owl:Class ;
              rdfs:subClassOf :Documentation ;
              rdfs:comment "A document providing information on an AI resource, meant to be used as assistive material to an oral/visual lecture on the resource."@en ;
              rdfs:label "Presentation"@en .


###  http://www.ai4eu.eu/ontologies/core#Publication
:Publication rdf:type owl:Class ;
             rdfs:subClassOf :KnowledgeComponent ;
             rdfs:comment "A published scholary manuscript."@en ;
             rdfs:label "Publication"@en .


###  http://www.ai4eu.eu/ontologies/core#Quality
:Quality rdf:type owl:Class ;
         rdfs:subClassOf :Entity ;
         rdfs:comment "A qualitative or descriptive characteristic of an AI-related entity."@en ;
         rdfs:label "Quality"@en .


###  http://www.ai4eu.eu/ontologies/core#Service
:Service rdf:type owl:Class ;
         rdfs:subClassOf :Distribution ;
         rdfs:comment "An AI resource distribution accessible as a web service."@en ;
         rdfs:label "Service"@en .


###  http://www.ai4eu.eu/ontologies/core#SoftwareComponent
:SoftwareComponent rdf:type owl:Class ;
                   rdfs:subClassOf :AIResource ;
                   rdfs:comment "A programmatic AI resource."@en ;
                   rdfs:label "Software Component"@en .


###  http://www.ai4eu.eu/ontologies/core#SourceCode
:SourceCode rdf:type owl:Class ;
            rdfs:subClassOf :Distribution ;
            rdfs:comment "The source code distribution of an AI resource"@en ;
            rdfs:label "Source Code"@en .


###  http://www.ai4eu.eu/ontologies/core#StandAlone
:StandAlone rdf:type owl:Class ;
            rdfs:subClassOf :Distribution ;
            rdfs:comment "A self-contained distribution of an AI resource."@en ;
            rdfs:label "StandAlone"@en .


###  http://www.ai4eu.eu/ontologies/core#SuccessStory
:SuccessStory rdf:type owl:Class ;
              rdfs:subClassOf :KnowledgeComponent ;
              rdfs:comment "A significant outcome, event or product"@en ;
              rdfs:label "Success Story"@en .


###  http://www.ai4eu.eu/ontologies/core#TechnologyReadinessLevel
:TechnologyReadinessLevel rdf:type owl:Class ;
                          rdfs:subClassOf :Quality ;
                          rdfs:comment "A metric denoting the maturity of a distribution of an AI resource."@en ;
                          rdfs:label "Technology Readiness Level"@en .


###  http://www.ai4eu.eu/ontologies/core#Tutorial
:Tutorial rdf:type owl:Class ;
          rdfs:subClassOf :Documentation ;
          rdfs:comment "A document that provides instructions on the usage of an AI resource on specific use cases and under a specific usage scenario."@en ;
          rdfs:label "Tutorial"@en .


###  http://www.ai4eu.eu/ontologies/core#Website
:Website rdf:type owl:Class ;
         rdfs:subClassOf :Documentation ;
         rdfs:comment "A group of web pages, under the same domain, partially or completely dedicated to an AI resource."@en ;
         rdfs:label "Website"@en .


###  http://www.ai4eu.eu/ontologies/core#Wiki
:Wiki rdf:type owl:Class ;
      rdfs:subClassOf :Website ;
      rdfs:comment "A collection of informative web pages dealing with different aspects of an AI resource and its usage."@en ;
      rdfs:label "Wiki"@en .


###  http://xmlns.com/foaf/0.1/Project
foaf:Project rdfs:subClassOf :KnowledgeComponent .


###  Generated by the OWL API (version 4.5.9.2019-02-01T07:24:44Z) https://github.com/owlcs/owlapi
